Uncomment

Gt3/Cotree/SimIx.lean
@@ -14,74 +14,74 @@ section MultiAddr
 variable
   [AddrVals μ₁ ι₁ (Node α₁ ι₁)] [AddrVals μ₂ ι₂ (Node α₂ ι₂)] [AddrVals μ₃ ι₃ (Node α₃ ι₃)]
 
-inductive SimIxRelUpto
+inductive SimIxUpto
   (stop : Prop) (rel : α₁ → α₂ → Prop) (lhs : μ₁) (rhs : μ₂) : ℕ → ι₁ → ι₂ → Prop
-  | done (i₁ i₂) : stop → SimIxRelUpto stop rel lhs rhs 0 i₁ i₂
+  | done (i₁ i₂) : stop → SimIxUpto stop rel lhs rhs 0 i₁ i₂
   | node {i₁ i₂ t₁ t₂}
     (hn₁ : t₁ ∈ getVals lhs i₁) (hn₂ : t₂ ∈ getVals rhs i₂)
     (tag : rel t₁.tag t₂.tag)
     (numChildren : numChildren t₁ = numChildren t₂)
     {gas}
     (children :
-      ∀ j, SimIxRelUpto stop rel lhs rhs gas
+      ∀ j, SimIxUpto stop rel lhs rhs gas
             (getChild t₁ j) (getChild t₂ (j.cast numChildren)))
-    : SimIxRelUpto stop rel lhs rhs (gas + 1) i₁ i₂
+    : SimIxUpto stop rel lhs rhs (gas + 1) i₁ i₂
 
-def SimIxRel (rel : α₁ → α₂ → Prop) (lhs : μ₁) (rhs : μ₂) (i₁ : ι₁) (i₂ : ι₂) : Prop
-  := ∀n, SimIxRelUpto ⊤ rel lhs rhs n i₁ i₂
+def SimIx (rel : α₁ → α₂ → Prop) (lhs : μ₁) (rhs : μ₂) (i₁ : ι₁) (i₂ : ι₂) : Prop
+  := ∀n, SimIxUpto ⊤ rel lhs rhs n i₁ i₂
 
-inductive TreeSimIxRel
+inductive TreeSimIx
   (rel : α₁ → α₂ → Prop) (lhs : μ₁) (rhs : μ₂) : ι₁ → ι₂ → Prop
   | node {i₁ i₂ t₁ t₂}
     (hn₁ : t₁ ∈ getVals lhs i₁) (hn₂ : t₂ ∈ getVals rhs i₂)
     (tag : rel t₁.tag t₂.tag)
     (numChildren : numChildren t₁ = numChildren t₂)
     (children :
-      ∀ j, TreeSimIxRel rel lhs rhs
+      ∀ j, TreeSimIx rel lhs rhs
             (getChild t₁ j) (getChild t₂ (j.cast numChildren)))
-    : TreeSimIxRel rel lhs rhs i₁ i₂
+    : TreeSimIx rel lhs rhs i₁ i₂
 
 variable
   {stop gas} {rel rel₁ rel₂ : α₁ → α₂ → Prop} {lhs : μ₁} {rhs : μ₂} {i₁ : ι₁} {i₂ : ι₂} {n₁ n₂}
 
-theorem SimIxRelUpto.anti_gas
+theorem SimIxUpto.anti_gas
   {gas₁ gas₂} (h : gas₁ ≤ gas₂) {i₁ : ι₁} {i₂ : ι₂}
-  (h : SimIxRelUpto ⊤ rel lhs rhs gas₂ i₁ i₂) : SimIxRelUpto ⊤ rel lhs rhs gas₁ i₁ i₂
+  (h : SimIxUpto ⊤ rel lhs rhs gas₂ i₁ i₂) : SimIxUpto ⊤ rel lhs rhs gas₁ i₁ i₂
   := match h, gas₁ with
   | _, 0 => .done i₁ i₂ trivial
   | .node hn₁ hn₂ h_tag h_numChildren h_children, gas₁ + 1 =>
     .node hn₁ hn₂ h_tag h_numChildren
       (fun j => anti_gas (by convert h using 0; simp) (h_children j))
 
-theorem SimIxRel.node
+theorem SimIx.node
   (hn₁ : n₁ ∈ getVals lhs i₁) (hn₂ : n₂ ∈ getVals rhs i₂)
   (tag : rel n₁.tag n₂.tag)
   (numChildren : numChildren n₁.tag = numChildren n₂.tag)
   (children :
-    ∀ j, SimIxRel (ι₁ := ι₁) (ι₂ := ι₂) rel lhs rhs
+    ∀ j, SimIx (ι₁ := ι₁) (ι₂ := ι₂) rel lhs rhs
           (getChild n₁ j) (getChild n₂ (j.cast numChildren)))
-  : SimIxRel rel lhs rhs i₁ i₂
+  : SimIx rel lhs rhs i₁ i₂
   | 0 => .done i₁ i₂ trivial
   | n + 1 => .node hn₁ hn₂ tag numChildren (fun j => children j n)
 
-theorem SimIxRelUpto.notBot : SimIxRelUpto stop ⊥ lhs rhs (gas + 1) i₁ i₂ → False
+theorem SimIxUpto.notBot : SimIxUpto stop ⊥ lhs rhs (gas + 1) i₁ i₂ → False
   | .node _ _ h_tag _ _ => by cases h_tag
 
-theorem SimIxRelUpto.ne_bot (h : SimIxRelUpto stop rel lhs rhs (gas + 1) i₁ i₂) : rel ≠ ⊥
+theorem SimIxUpto.ne_bot (h : SimIxUpto stop rel lhs rhs (gas + 1) i₁ i₂) : rel ≠ ⊥
   := fun e => (e ▸ h).notBot
 
-theorem SimIxRel.notBot (h : SimIxRel ⊥ lhs rhs i₁ i₂) : False := (h 1).notBot
+theorem SimIx.notBot (h : SimIx ⊥ lhs rhs i₁ i₂) : False := (h 1).notBot
 
-theorem SimIxRel.ne_bot (h : SimIxRel rel lhs rhs i₁ i₂) : rel ≠ ⊥ := (h 1).ne_bot
+theorem SimIx.ne_bot (h : SimIx rel lhs rhs i₁ i₂) : rel ≠ ⊥ := (h 1).ne_bot
 
-theorem SimIxRelUpto.mono_rel (hrel : rel₁ ≤ rel₂) {gas} {i₁ : ι₁} {i₂ : ι₂}
-  : SimIxRelUpto stop rel₁ lhs rhs gas i₁ i₂ → SimIxRelUpto stop rel₂ lhs rhs gas i₁ i₂
+theorem SimIxUpto.mono_rel (hrel : rel₁ ≤ rel₂) {gas} {i₁ : ι₁} {i₂ : ι₂}
+  : SimIxUpto stop rel₁ lhs rhs gas i₁ i₂ → SimIxUpto stop rel₂ lhs rhs gas i₁ i₂
   | .done _ _ hs => .done i₁ i₂ hs
   | .node hn₁ hn₂ h_tag h_numChildren h_children =>
     .node hn₁ hn₂ (hrel _ _ h_tag) h_numChildren (fun j => mono_rel hrel (h_children j))
 
-theorem SimIxRel.mono_rel (hrel : rel₁ ≤ rel₂) {i₁ : ι₁} {i₂ : ι₂} (h : SimIxRel rel₁ lhs rhs i₁ i₂)
-  : SimIxRel rel₂ lhs rhs i₁ i₂ := fun n => (h n).mono_rel hrel
+theorem SimIx.mono_rel (hrel : rel₁ ≤ rel₂) {i₁ : ι₁} {i₂ : ι₂} (h : SimIx rel₁ lhs rhs i₁ i₂)
+  : SimIx rel₂ lhs rhs i₁ i₂ := fun n => (h n).mono_rel hrel
 
 section GTrans
 
@@ -89,14 +89,14 @@ variable
   {rel₁ : α₁ → α₂ → Prop} {rel₂ : α₂ → α₃ → Prop} {rel₃ : α₁ → α₃ → Prop}
   {lhs : μ₁} {mid : μ₂} {rhs : μ₃}
 
-theorem SimIxRelUpto.gtrans
+theorem SimIxUpto.gtrans
   [AddrVals.Det μ₁ ι₁ (Node α₁ ι₁)]
   [AddrVals.Det μ₂ ι₂ (Node α₂ ι₂)]
   [AddrVals.Det μ₃ ι₃ (Node α₃ ι₃)]
   (hrel : ∀ a b c, rel₁ a b → rel₂ b c → rel₃ a c)
   {gas} {i₁ : ι₁} {i₂ : ι₂} {i₃ : ι₃}
-  : SimIxRelUpto stop rel₁ lhs mid gas i₁ i₂ → SimIxRelUpto stop rel₂ mid rhs gas i₂ i₃
-    → SimIxRelUpto stop rel₃ lhs rhs gas i₁ i₃
+  : SimIxUpto stop rel₁ lhs mid gas i₁ i₂ → SimIxUpto stop rel₂ mid rhs gas i₂ i₃
+    → SimIxUpto stop rel₃ lhs rhs gas i₁ i₃
   | .done _ _ hs, .done _ _ _ => .done i₁ i₃ hs
   | .node hn₁ hn₂ h1_tag h1_numChildren h1_children,
     .node hn₂' hn₃ h2_tag h2_numChildren h2_children => by
@@ -104,16 +104,16 @@ theorem SimIxRelUpto.gtrans
     exact .node hn₁ hn₃ (hrel _ _ _ h1_tag h2_tag) (h1_numChildren.trans h2_numChildren)
       (fun j => gtrans hrel (h1_children j) (h2_children (j.cast h1_numChildren)))
 
-theorem SimIxRel.gtrans
+theorem SimIx.gtrans
   [AddrVals.Det μ₁ ι₁ (Node α₁ ι₁)]
   [AddrVals.Det μ₂ ι₂ (Node α₂ ι₂)]
   [AddrVals.Det μ₃ ι₃ (Node α₃ ι₃)]
   (hrel : ∀ a b c, rel₁ a b → rel₂ b c → rel₃ a c)
   {i₁ : ι₁} {i₂ : ι₂} {i₃ : ι₃}
-  (h1 : SimIxRel rel₁ lhs mid i₁ i₂)
-  (h2 : SimIxRel rel₂ mid rhs i₂ i₃)
-  : SimIxRel rel₃ lhs rhs i₁ i₃
-  := fun n => SimIxRelUpto.gtrans hrel (h1 n) (h2 n)
+  (h1 : SimIx rel₁ lhs mid i₁ i₂)
+  (h2 : SimIx rel₂ mid rhs i₂ i₃)
+  : SimIx rel₃ lhs rhs i₁ i₃
+  := fun n => SimIxUpto.gtrans hrel (h1 n) (h2 n)
 
 end GTrans
 
@@ -130,51 +130,51 @@ variable
   {rel : α → α → Prop}
   {addr : μ} {lhs : μ₁} {rhs : μ₂}
 
-theorem SimIxRelUpto.refl
+theorem SimIxUpto.refl
   [IsRefl α rel] [AddrVals.Inhab μ ι (Node α ι)]
-  {gas} (i : ι) : SimIxRelUpto ⊤ rel addr addr gas i i
+  {gas} (i : ι) : SimIxUpto ⊤ rel addr addr gas i i
   := match gas with
   | 0 => .done i i trivial
   | _ + 1 =>
     have ⟨y, hy⟩ := AddrVals.Inhab.inhab addr i;
     .node hy hy (IsRefl.refl _) rfl (fun j => refl (getChild y j))
 
-theorem SimIxRel.refl
-  [IsRefl α rel] [AddrVals.Inhab μ ι (Node α ι)] (i : ι) : SimIxRel rel addr addr i i
+theorem SimIx.refl
+  [IsRefl α rel] [AddrVals.Inhab μ ι (Node α ι)] (i : ι) : SimIx rel addr addr i i
   := fun _ => .refl i
 
-theorem SimIxRelUpto.symm [IsSymm α rel]
+theorem SimIxUpto.symm [IsSymm α rel]
   {gas} {i₁ : ι₁} {i₂ : ι₂}
-  : SimIxRelUpto stop rel lhs rhs gas i₁ i₂ → SimIxRelUpto stop rel rhs lhs gas i₂ i₁
+  : SimIxUpto stop rel lhs rhs gas i₁ i₂ → SimIxUpto stop rel rhs lhs gas i₂ i₁
   | .done _ _ hs => .done i₂ i₁ hs
   | .node hn₁ hn₂ h_tag h_numChildren h_children =>
     .node hn₂ hn₁ (IsSymm.symm _ _ h_tag) h_numChildren.symm
       (fun j => symm (h_children (j.cast (Eq.symm h_numChildren))))
 
-theorem SimIxRel.symm {rel} [IsSymm α rel]
-  {i₁ : ι₁} {i₂ : ι₂} (h : SimIxRel rel lhs rhs i₁ i₂) : SimIxRel rel rhs lhs i₂ i₁
+theorem SimIx.symm {rel} [IsSymm α rel]
+  {i₁ : ι₁} {i₂ : ι₂} (h : SimIx rel lhs rhs i₁ i₂) : SimIx rel rhs lhs i₂ i₁
   := fun n => (h n).symm
 
 variable
   {lhs : μ₁} {mid : μ₂} {rhs : μ₃}
 
-theorem SimIxRelUpto.trans {rel} [IsTrans α rel]
+theorem SimIxUpto.trans {rel} [IsTrans α rel]
   [AddrVals.Det μ₁ ι₁ (Node α ι₁)]
   [AddrVals.Det μ₂ ι₂ (Node α ι₂)]
   [AddrVals.Det μ₃ ι₃ (Node α ι₃)]
   {gas} {i₁ : ι₁} {i₂ : ι₂} {i₃ : ι₃}
-  (h1 : SimIxRelUpto stop rel lhs mid gas i₁ i₂)
-  (h2 : SimIxRelUpto stop rel mid rhs gas i₂ i₃)
-  : SimIxRelUpto stop rel lhs rhs gas i₁ i₃
+  (h1 : SimIxUpto stop rel lhs mid gas i₁ i₂)
+  (h2 : SimIxUpto stop rel mid rhs gas i₂ i₃)
+  : SimIxUpto stop rel lhs rhs gas i₁ i₃
   := h1.gtrans IsTrans.trans h2
 
-theorem SimIxRel.trans {rel} [IsTrans α rel]
+theorem SimIx.trans {rel} [IsTrans α rel]
   [AddrVals.Det μ₁ ι₁ (Node α ι₁)]
   [AddrVals.Det μ₂ ι₂ (Node α ι₂)]
   [AddrVals.Det μ₃ ι₃ (Node α ι₃)] {i₁ : ι₁} {i₂ : ι₂} {i₃ : ι₃}
-  (h1 : SimIxRel rel lhs mid i₁ i₂)
-  (h2 : SimIxRel rel mid rhs i₂ i₃)
-  : SimIxRel rel lhs rhs i₁ i₃
+  (h1 : SimIx rel lhs mid i₁ i₂)
+  (h2 : SimIx rel mid rhs i₂ i₃)
+  : SimIx rel lhs rhs i₁ i₃
   := h1.gtrans IsTrans.trans h2
 
 end SingleAddr
