Gt3/Graph/Basic.lean
@@ -1,0 +1,11 @@
+import Gt3.Tree.Node
+import Gt3.Cotree.SimIx
+
+namespace Gt3
+
+open NumChildren BinderList HasChildren FlatChildren
+
+structure Graph (ι : Type _) (α : Type _) [NumChildren α] where
+  nodes : ι → Node α ι
+
+end Gt3
